<?xml version="1.0"?>
<rdf:RDF
    xmlns:rdf="http://www.w3.org/1999/02/22-rdf-syntax-ns#"
    xmlns:lemon="http://lemon-model.net/lemon#"
    xmlns:protege="http://protege.stanford.edu/plugins/owl/protege#"
    xmlns:xsp="http://www.owl-ontologies.com/2005/08/07/xsp.owl#"
    xmlns:dbnary="http://kaiko.getalp.org/dbnary#"
    xmlns:owl="http://www.w3.org/2002/07/owl#"
    xmlns:dcterms="http://purl.org/dc/terms/"
    xmlns:xsd="http://www.w3.org/2001/XMLSchema#"
    xmlns:swrl="http://www.w3.org/2003/11/swrl#"
    xmlns:swrlb="http://www.w3.org/2003/11/swrlb#"
    xmlns:rdfs="http://www.w3.org/2000/01/rdf-schema#"
  xml:base="http://kaiko.getalp.org/dbnary">
  <owl:Ontology rdf:about="">
    <rdfs:seeAlso rdf:datatype="http://www.w3.org/2001/XMLSchema#string"
    >http://kaiko.getalp.org/about-dbnary/</rdfs:seeAlso>
    <owl:imports rdf:resource="http://lemon-model.net/lemon"/>
    <rdfs:label rdf:datatype="http://www.w3.org/2001/XMLSchema#string"
    >dbnary</rdfs:label>
    <rdfs:comment xml:lang="en">DBnary: A lexicon model designed to allow the representation of lexical data extracted from wiktionary language editions (http://www.wiktionary.org/). The dbnary model extends the lemon model (http://lemon-model.net/lemon).</rdfs:comment>
  </owl:Ontology>
  <owl:Class rdf:ID="Translation">
    <rdfs:comment xml:lang="en">Describe translation information for a Lexical Entry or a Lexical Sense.</rdfs:comment>
  </owl:Class>
  <owl:Class rdf:about="http://purl.org/dc/terms/LinguisticSystem"/>
  <owl:Class rdf:about="http://lemon-model.net/lemon#LexicalEntry"/>
  <owl:Class rdf:ID="LexicalEntity">
    <owl:disjointUnionOf rdf:parseType="Collection">
      <owl:Class rdf:about="http://lemon-model.net/lemon#LexicalEntry"/>
      <owl:Class rdf:about="http://lemon-model.net/lemon#LexicalSense"/>
    </owl:disjointUnionOf>
    <rdfs:subClassOf>
      <owl:Class rdf:about="http://lemon-model.net/lemon#LemonElement"/>
    </rdfs:subClassOf>
  </owl:Class>
  <owl:Class rdf:ID="Vocable">
    <rdfs:subClassOf rdf:resource="http://lemon-model.net/lemon#LexicalEntry"/>
    <rdfs:comment xml:lang="en">A Vocable corresponds to a set of Lexical Entries that usually share the same written form but that do not necessarily share the same Part Of Speech. E.g. cat_n and cat_v are distinct lexical entries while the vocable "cat" refers to both of them.</rdfs:comment>
  </owl:Class>
  <owl:Class rdf:ID="EtymologyEntry">
    <rdfs:comment xml:lang="en">An EtymologyEntry corresponds to a set of Lexical Entries that share the same etymology but that do not necessarily share the same Part Of Speech. E.g. eng:link_n_1 and eng:link_v_1 are distinct lexical entries and the etymology entry link_ety_1 refers to both of them because link_n_1 and link_v_1 share the same etymology from Old English ang:linke.</rdfs:comment>
    <rdfs:subClassOf rdf:resource="http://lemon-model.net/lemon#LexicalEntry"/>
  </owl:Class>
  <owl:ObjectProperty rdf:ID="meronym">
    <rdfs:comment xml:lang="en">An underspecified meronymy relation between LexicalEntities (Lexical entries or Lexical Senses). This relation is used to encode an information available in a lexicon when the linked Lexical Senses are not known. When both source and target of the relation are Lexical Senses, one should use the corresponding LEMON relation. </rdfs:comment>
    <rdfs:subPropertyOf>
      <owl:ObjectProperty rdf:ID="topNymProperty"/>
    </rdfs:subPropertyOf>
  </owl:ObjectProperty>
  <owl:ObjectProperty rdf:ID="derivesFrom">
    <rdfs:subPropertyOf>
      <owl:ObjectProperty rdf:ID="etymologicallyRelatedTo"/>
    </rdfs:subPropertyOf>
    <rdfs:domain rdf:resource="#LexicalEntry"/>
    <rdfs:comment xml:lang="en">The target LexicalEntry is a term derived from the source LexicalEntry. E.g.:eng:link_up derivesFrom eng:link_ety_1. </rdfs:comment>
    <rdfs:range rdf:resource="#LexicalEntry"/>
  </owl:ObjectProperty>
  <owl:ObjectProperty rdf:ID="approximateSynonym">
    <rdfs:comment xml:lang="en">An underspecified approximate synonymy relation between LexicalEntities (Lexical entries or Lexical Senses). This relation is used to encode an information available in a lexicon when the linked Lexical Senses are not known. When both source and target of the relation are Lexical Senses, one should use the corresponding LEMON relation. </rdfs:comment>
    <rdfs:subPropertyOf>
      <owl:ObjectProperty rdf:about="#topNymProperty"/>
    </rdfs:subPropertyOf>
  </owl:ObjectProperty>
  <owl:ObjectProperty rdf:ID="refersTo">
    <rdfs:domain rdf:resource="#Vocable"/>
    <rdfs:comment xml:lang="en">links a vocable to any lexical entry that share the same written form. </rdfs:comment>
    <rdfs:range rdf:resource="http://lemon-model.net/lemon#LexicalEntry"/>
  </owl:ObjectProperty>
  <owl:ObjectProperty rdf:ID="synonym">
    <rdfs:comment xml:lang="en">An underspecified synonymy relation between LexicalEntities (Lexical entries or Lexical Senses). This relation is used to encode an information available in a lexicon when the linked Lexical Senses are not known. When both source and target of the relation are Lexical Senses, one should use the corresponding LEMON relation. </rdfs:comment>
    <rdfs:subPropertyOf>
      <owl:ObjectProperty rdf:about="#topNymProperty"/>
    </rdfs:subPropertyOf>
  </owl:ObjectProperty>
  <owl:ObjectProperty rdf:about="#topNymProperty">
    <rdfs:range rdf:resource="#LexicalEntity"/>
    <rdfs:domain rdf:resource="#LexicalEntity"/>
    <rdfs:comment xml:lang="en">An underspecified lexico semantic relation between LexicalEntities (Lexical entry OR Lexical Sense). This relation is used to encode an information available in a lexicon when the linked Lexical Senses are not known. When both source and target of the relation are Lexical Senses, one should use the corresponding LEMON relation. </rdfs:comment>
  </owl:ObjectProperty>
  <owl:ObjectProperty rdf:about="#etymologicallyRelatedTo">
    <rdfs:range rdf:resource="#LexicalEntry"/>
    <rdfs:comment xml:lang="en">An underspecified etymological relationship betwen two LexicalEntries. </rdfs:comment>
    <rdfs:domain rdf:resource="#LexicalEntry"/>
  </owl:ObjectProperty>
  <owl:ObjectProperty rdf:ID="descendsFrom">
    <rdfs:domain rdf:resource="#LexicalEntry"/>
    <rdfs:subPropertyOf rdf:resource="#etymologicallyRelatedTo"/>
    <rdfs:range rdf:resource="#LexicalEntry"/>
    <rdfs:comment xml:lang="en">The target LexicalEntry is a descendant of the source LexicalEntry. </rdfs:comment>
  </owl:ObjectProperty>
  <owl:ObjectProperty rdf:ID="hyponym">
    <rdfs:comment xml:lang="en">An underspecified hyponymy relation between LexicalEntities (Lexical entries or Lexical Senses). This relation is used to encode an information available in a lexicon when the linked Lexical Senses are not known. When both source and target of the relation are Lexical Senses, one should use the corresponding LEMON relation. </rdfs:comment>
    <rdfs:subPropertyOf rdf:resource="#topNymProperty"/>
  </owl:ObjectProperty>
  <owl:ObjectProperty rdf:ID="holonym">
    <rdfs:subPropertyOf rdf:resource="#topNymProperty"/>
    <rdfs:comment xml:lang="en">An underspecified holonymy relation between LexicalEntities (Lexical entries or Lexical Senses). This relation is used to encode an information available in a lexicon when the linked Lexical Senses are not known. When both source and target of the relation are Lexical Senses, one should use the corresponding LEMON relation. </rdfs:comment>
  </owl:ObjectProperty>
  <owl:ObjectProperty rdf:ID="troponym">
    <rdfs:subPropertyOf rdf:resource="#topNymProperty"/>
    <rdfs:comment xml:lang="en">A verb that indicates more precisely the manner of doing something by replacing a verb of a more generalized meaning. E.g.: "Stroll" is a troponym of "walk", since it involves a slow and relaxed sort of walking.</rdfs:comment>
  </owl:ObjectProperty>
  <owl:ObjectProperty rdf:ID="isTranslationOf">
    <rdfs:domain rdf:resource="#Translation"/>
    <rdfs:comment xml:lang="en">links the translation information to the Lexical Entity it belongs to.</rdfs:comment>
    <rdfs:range rdf:resource="#LexicalEntity"/>
  </owl:ObjectProperty>
  <owl:ObjectProperty rdf:ID="etymologicallyDerivesFrom">
    <rdfs:range rdf:resource="#LexicalEntry"/>
    <rdfs:subPropertyOf rdf:resource="#etymologicallyRelatedTo"/>
    <rdfs:comment xml:lang="en">The target LexicalEntry etymologically derives from the source LexicalEntry. </rdfs:comment>
    <rdfs:domain rdf:resource="#LexicalEntry"/>
  </owl:ObjectProperty>
  <owl:ObjectProperty rdf:ID="hypernym">
    <rdfs:comment xml:lang="en">An underspecified hypernymy relation between LexicalEntities (Lexical entries or Lexical Senses). This relation is used to encode an information available in a lexicon when the linked Lexical Senses are not known. When both source and target of the relation are Lexical Senses, one should use the corresponding LEMON relation. </rdfs:comment>
    <rdfs:subPropertyOf rdf:resource="#topNymProperty"/>
  </owl:ObjectProperty>
  <owl:ObjectProperty rdf:ID="antonym">
    <rdfs:subPropertyOf rdf:resource="#topNymProperty"/>
    <rdfs:comment xml:lang="en">An underspecified antonymy relation between LexicalEntities (Lexical entries or Lexical Senses). This relation is used to encode an information available in a lexicon when the linked Lexical Senses are not known. When both source and target of the relation are Lexical Senses, one should use the corresponding LEMON relation. </rdfs:comment>
  </owl:ObjectProperty>
  <owl:ObjectProperty rdf:ID="etymologicallyEquivalentTo">
    <rdfs:comment xml:lang="en">The target and the source LexicalEntries share the same etymological origin. </rdfs:comment>
    <rdfs:domain rdf:resource="#LexicalEntry"/>
    <rdfs:subPropertyOf rdf:resource="#etymologicallyRelatedTo"/>
    <rdfs:range rdf:resource="#LexicalEntry"/>
  </owl:ObjectProperty>
  <rdf:Property rdf:about="http://www.w3.org/2002/07/owl#topObjectProperty"/>
  <owl:DatatypeProperty rdf:ID="writtenForm">
    <rdfs:domain rdf:resource="#Translation"/>
    <rdfs:range rdf:resource="http://www.w3.org/2001/XMLSchema#string"/>
    <rdfs:comment xml:lang="en">The written form of a translation equivalent.</rdfs:comment>
  </owl:DatatypeProperty>
  <owl:DatatypeProperty rdf:ID="senseNumber">
    <rdfs:comment xml:lang="en">The number of the lexical Sense in the Lexical Entry, as given by Wiktionary. This property takes a String literal as an object.</rdfs:comment>
  </owl:DatatypeProperty>
  <owl:DatatypeProperty rdf:ID="partOfSpeech">
    <rdfs:domain rdf:resource="http://lemon-model.net/lemon#LexicalEntry"/>
    <rdfs:range rdf:resource="http://www.w3.org/2001/XMLSchema#string"/>
    <rdfs:comment xml:lang="en">The original part of speech as it was defined in the Wiktionary page. This property takes a String literal as object.</rdfs:comment>
  </owl:DatatypeProperty>
  <owl:DatatypeProperty rdf:ID="note">
    <rdfs:range rdf:resource="http://www.w3.org/2001/XMLSchema#string"/>
    <rdfs:domain rdf:resource="http://lemon-model.net/lemon#LemonElement"/>
    <rdfs:comment xml:lang="en">Textual note that may be used to add information to a LemonElement when no standard vocabularies exists to explicit it.</rdfs:comment>
  </owl:DatatypeProperty>
  <owl:DatatypeProperty rdf:ID="gloss">
    <rdfs:comment xml:lang="en">A textual gloss that may be used to disambiguate the translation's source sense. </rdfs:comment>
    <rdfs:domain rdf:resource="#Translation"/>
    <rdfs:range rdf:resource="http://www.w3.org/2001/XMLSchema#string"/>
  </owl:DatatypeProperty>
  <owl:DatatypeProperty rdf:ID="usage">
    <rdfs:range rdf:resource="http://www.w3.org/2001/XMLSchema#string"/>
    <rdfs:domain rdf:resource="#Translation"/>
    <rdfs:comment xml:lang="en">Usage note that is used to further annotate the target of the translation.</rdfs:comment>
  </owl:DatatypeProperty>
  <owl:DatatypeProperty rdf:ID="exampleSource">
    <rdf:type rdf:resource="http://www.w3.org/2002/07/owl#AnnotationProperty"/>
    <rdfs:domain rdf:resource="http://lemon-model.net/lemon#UsageExample"/>
  </owl:DatatypeProperty>
  <owl:FunctionalProperty rdf:ID="targetLanguage">
    <rdf:type rdf:resource="http://www.w3.org/2002/07/owl#ObjectProperty"/>
    <rdfs:range rdf:resource="http://purl.org/dc/terms/LinguisticSystem"/>
    <rdfs:comment xml:lang="en">The target language of a given translation, defined as a Linguistic System.</rdfs:comment>
    <rdfs:domain rdf:resource="#Translation"/>
  </owl:FunctionalProperty>
  <owl:FunctionalProperty rdf:ID="targetLanguageCode">
    <rdfs:domain rdf:resource="#Translation"/>
    <rdf:type rdf:resource="http://www.w3.org/2002/07/owl#DatatypeProperty"/>
    <rdfs:range rdf:resource="http://www.w3.org/2001/XMLSchema#string"/>
    <rdfs:comment xml:lang="en">The target language of a given translation. This may be used when the dbnary:targetLanguage object property can not be used.</rdfs:comment>
  </owl:FunctionalProperty>
</rdf:RDF>

<!-- Created with Protege (with OWL Plugin 3.4.1, Build 536)  http://protege.stanford.edu -->
